src/ByteStringFMap.v
@@ -1,0 +1,299 @@
+Require Import
+  Coq.Lists.List
+  Coq.Arith.Arith
+  Coq.NArith.NArith
+  Fiat.ADT
+  Fiat.ADTNotation
+  Fiat.ADTRefinement
+  Fiat.ADTRefinement.BuildADTRefinements
+  ByteString.ADTInduction
+  ByteString.BindDep
+  ByteString.ByteString
+  ByteString.ByteStringHeap
+  ByteString.Memory
+  ByteString.Heap
+  ByteString.Nomega
+  ByteString.Relations
+  ByteString.Tactics
+  Coq.FSets.FMapFacts
+  Coq.Structures.DecidableTypeEx.
+
+Generalizable All Variables.
+
+Module ByteStringFMap (M : WSfun N_as_DT).
+
+Module Import ByteStringHeap := ByteStringHeap M.
+Import HeapCanonical.
+Import HeapCanonical.HeapADT.
+Import HeapCanonical.HeapADT.Heap.
+Import HeapCanonical.HeapADT.Heap.FMapExt.
+Import HeapCanonical.HeapADT.Heap.FMapExt.P.
+Import HeapCanonical.HeapADT.Heap.FMapExt.F.
+
+Section Refined.
+
+Definition cHeapRep := ComputationalADT.cRep (projT1 HeapCanonical).
+
+Variable heap  : Rep HSpec.
+Variable heap' : cHeapRep.
+
+Definition Heap_AbsR (or : Rep HeapSpec) nr :=
+  M.Equal (resvs or) (resvs (snd nr)) /\
+  M.Equal (bytes or) (bytes (snd nr)) /\
+  P.for_all (within_allocated_mem (fst nr)) (resvs (snd nr)).
+
+Variable heap_AbsR : Heap_AbsR (` heap) heap'.
+
+(* This style of computational refinement makes use of a separately refined
+   heap. Another approach is to refine the heap methods directly, which would
+   mean going directly to the metal (but would require replicating much of the
+   proof word that is done in HeapFMap.v). *)
+
+Record PS' := {
+  ps'Heap : cHeapRep;
+
+  ps'Buffer : N;
+  ps'BufLen : N;
+
+  ps'Offset : N;
+  ps'Length : N
+}.
+
+Lemma ByteStringImpl : FullySharpened (projT1 (ByteStringHeap heap)).
+Proof.
+  start sharpening ADT.
+
+  hone representation using
+       (fun (or : PS) (nr : PS') =>
+          Heap_AbsR (` (psHeap or)) (ps'Heap nr) /\
+          psBuffer or = ps'Buffer nr /\
+          psBufLen or = ps'BufLen nr /\
+          psOffset or = ps'Offset nr /\
+          psLength or = ps'Length nr);
+
+  try simplify with monad laws; simpl.
+  {
+    refine pick val {| ps'Heap   := heap'
+                     ; ps'Buffer := 0
+                     ; ps'BufLen := 0
+                     ; ps'Offset := 0
+                     ; ps'Length := 0 |}.
+      finish honing.
+    simpl; intuition.
+  }
+  {
+    repeat match goal with
+      [ H : _ /\ _ |- _ ] => destruct H
+    end; subst.
+    destruct r_o, psHeap; simpl in *.
+    rewrite H1, H2, H3, H4.
+    rewrite refineEquiv_If_Then_Else_Bind.
+    apply refine_If_Then_Else.
+      simplify with monad laws; simpl.
+      unfold poke'; simpl.
+      remove_dependency; simpl.
+      unfold poke.
+      simplify with monad laws; simpl.
+      refine pick val
+             {| ps'Heap   :=
+                  (fst (ps'Heap r_n),
+                   {| resvs := resvs (snd (ps'Heap r_n))
+                    ; bytes := M.add (ps'Buffer r_n + (ps'Offset r_n - 1)) d
+                                     (bytes (snd (ps'Heap r_n))) |})
+              ; ps'Buffer := ps'Buffer r_n
+              ; ps'BufLen := ps'BufLen r_n
+              ; ps'Offset := ps'Offset r_n - 1
+              ; ps'Length := ps'Length r_n + 1 |}.
+        simplify with monad laws.
+        finish honing.
+      simpl in *; intuition.
+      destruct H0, H5.
+      split; simpl; trivial.
+      split; trivial.
+      apply add_m; eauto.
+    rewrite refineEquiv_If_Then_Else_Bind.
+    subst H.
+    apply refine_If_Then_Else.
+      simplify with monad laws; simpl.
+      unfold memcpy', poke'; simpl.
+      remove_dependency; simpl.
+      setoid_rewrite refine_bind_dep_bind_ret; simpl.
+      do 2 setoid_rewrite refine_bind_dep_ignore.
+      unfold memcpy, poke.
+      simplify with monad laws; simpl.
+      refine pick val
+             {| ps'Heap   :=
+                  (fst (ps'Heap r_n),
+                   {| resvs := resvs (snd (ps'Heap r_n))
+                    ; bytes :=
+                        M.add (ps'Buffer r_n + 0) d
+                              (copy_bytes (ps'Buffer r_n) (ps'Buffer r_n + 1)
+                                          (ps'Length r_n)
+                                          (bytes (snd (ps'Heap r_n)))) |})
+              ; ps'Buffer := ps'Buffer r_n
+              ; ps'BufLen := ps'BufLen r_n
+              ; ps'Offset := 0
+              ; ps'Length := ps'Length r_n + 1 |}.
+        simplify with monad laws.
+        finish honing.
+      simpl in *; intuition.
+      destruct H0, H0.
+      split; simpl; trivial.
+      split; trivial.
+      apply add_m; auto.
+      rewrite H0; reflexivity.
+    rewrite refineEquiv_If_Then_Else_Bind.
+    apply refine_If_Then_Else.
+      simplify with monad laws; simpl.
+      unfold alloc', memcpy', poke'.
+      remove_dependency; simpl.
+      do 3 setoid_rewrite refine_bind_dep_bind_ret.
+      simpl; remove_dependency.
+      do 3 setoid_rewrite refine_bind_dep_ignore.
+      unfold ByteStringHeap.buffer_cons_obligation_2.
+      unfold alloc, memcpy, free, poke, find_free_block.
+      simplify with monad laws; simpl.
+      refine pick val (fst (ps'Heap r_n)).
+        simplify with monad laws; simpl.
+        refine pick val
+               {| ps'Heap   :=
+                    (fst (ps'Heap r_n) + ps'Length r_n + alloc_quantum,
+                     {| resvs :=
+                          M.remove (ps'Buffer r_n)
+                                   (M.add (fst (ps'Heap r_n))
+                                          (ps'Length r_n + 1)
+                                          (resvs (snd (ps'Heap r_n))))
+                      ; bytes :=
+                          M.add (fst (ps'Heap r_n) + 0) d
+                                (copy_bytes (ps'Buffer r_n)
+                                            (fst (ps'Heap r_n) + 1)
+                                            (ps'Length r_n)
+                                            (bytes (snd (ps'Heap r_n)))) |})
+                ; ps'Buffer := fst (ps'Heap r_n)
+                ; ps'BufLen := ps'Length r_n + alloc_quantum
+                ; ps'Offset := 0
+                ; ps'Length := ps'Length r_n + alloc_quantum |}.
+          simplify with monad laws.
+          finish honing.
+        simpl in *; intuition.
+        destruct H0, H0.
+        split; simpl.
+           rewrite H; reflexivity.
+        split.
+          rewrite H0; reflexivity.
+        rewrite <- remove_add.
+        apply for_all_remove; relational.
+        apply for_all_add_true; relational.
+          simplify_maps.
+        split.
+          apply for_all_remove; relational.
+          eapply for_all_impl; auto; relational.
+            exact H5.
+          intros.
+          unfold within_allocated_mem in *.
+          nomega.
+        nomega.
+      destruct H0, H0.
+      rewrite H.
+      eapply for_all_impl; eauto; relational.
+      intros.
+      unfold within_allocated_mem in *.
+      nomega.
+    unfold allocate_buffer, alloc', poke'.
+    remove_dependency; simpl.
+    unfold Bind2.
+    rewrite refine_bind_bind.
+    remove_dependency.
+    setoid_rewrite refine_bind_dep_bind_ret.
+    autorewrite with monad laws; simpl.
+    remove_dependency.
+    setoid_rewrite refine_bind_dep_ignore.
+    unfold alloc, find_free_block.
+    simplify with monad laws; simpl.
+    refine pick val (fst (ps'Heap r_n)).
+      simplify with monad laws; simpl.
+      refine pick val
+             {| ps'Heap   :=
+                  (fst (ps'Heap r_n) + 1,
+                   {| resvs := M.add (fst (ps'Heap r_n)) 1
+                                     (resvs (snd (ps'Heap r_n)))
+                    ; bytes := M.add (fst (ps'Heap r_n) + 0) d
+                                     (bytes (snd (ps'Heap r_n))) |})
+              ; ps'Buffer := fst (ps'Heap r_n)
+              ; ps'BufLen := 1
+              ; ps'Offset := 0
+              ; ps'Length := 1 |}.
+        simplify with monad laws.
+        finish honing.
+      simpl in *; intuition.
+      destruct H0, H0.
+      split; simpl.
+        rewrite H; reflexivity.
+      split.
+        rewrite H0; reflexivity.
+      rewrite <- remove_add.
+      apply for_all_add_true; relational.
+        simplify_maps.
+      split.
+        apply for_all_remove; relational.
+        eapply for_all_impl; auto; relational.
+          exact H5.
+        intros.
+        unfold within_allocated_mem in *.
+        nomega.
+      nomega.
+    destruct H0, H0.
+    rewrite H.
+    eapply for_all_impl; eauto; relational.
+    intros.
+    unfold within_allocated_mem in *.
+    nomega.
+  }
+  {
+    repeat match goal with
+      [ H : _ /\ _ |- _ ] => destruct H
+    end; subst.
+    rewrite H1, H2, H3, H4.
+    rewrite refineEquiv_If_Then_Else_Bind.
+    subst H.
+    apply refine_If_Then_Else.
+      simplify with monad laws; simpl.
+      unfold peek'.
+      remove_dependency.
+      unfold peek.
+      simplify with monad laws; simpl.
+      refine pick val (Ifopt M.find (ps'Buffer r_n + ps'Offset r_n)
+                                    (bytes (snd (ps'Heap r_n))) as v
+                       Then v
+                       Else Zero).
+        simplify with monad laws; simpl.
+        refine pick val {| ps'Heap   := ps'Heap r_n
+                         ; ps'Buffer := ps'Buffer r_n
+                         ; ps'BufLen := ps'BufLen r_n
+                         ; ps'Offset := if ps'Length r_n =? 1
+                                        then 0
+                                        else ps'Offset r_n + 1
+                         ; ps'Length := ps'Length r_n - 1 |}.
+          simplify with monad laws.
+          finish honing.
+        simpl in *; intuition.
+      intros.
+      destruct H0, H5.
+      destruct (M.find _ _) eqn:Heqe; simpl.
+        rewrite H5 in H.
+        normalize.
+        eapply F.MapsTo_fun; eauto.
+      apply F.find_mapsto_iff in H.
+      congruence.
+    simplify with monad laws; simpl.
+    refine pick val r_n.
+      simplify with monad laws; simpl.
+      finish honing.
+    intuition.
+  }
+  finish_SharpeningADT_WithoutDelegation.
+Defined.
+
+End Refined.
+
+End ByteStringFMap.
